\documentclass{article}
\usepackage{parskip}
\usepackage[utf8]{inputenc}
\usepackage{fullpage}
\setlength{\parskip}{0.7cm}

\begin{document}
\section{Task}
\par Given: \newline
$R(a, b, c, d, e)$ \newline
$F = \{  
        a \rightarrow c,
        bc \rightarrow d,
        d \rightarrow a,
        b \rightarrow e
    \}$
\par
$a^{+} = \{a, c \}$ \newline
$b^{+} = \{b, e \}$ \newline
$c^{+} = \{c \}$ \newline
$d^{+} = \{a, c, d \}$ \newline
$e^{+} = \{e \}$ \newline
$\Rightarrow$ no key: try subsets with two attributes

\par
$ab^{+} = \{a, b, c, d, e \}$ \newline
$ac^{+} = \{a, c \}$ \newline
$ad^{+} = \{a, c, d \}$ \newline
$ae^{+} = \{a, c, e \}$ \newline
$bc^{+} = \{a, b, c, d, e \}$ \newline
$bd^{+} = \{a, b, c, d, e \}$ \newline
$be^{+} = \{b, e \}$ \newline
$cd^{+} = \{a, c, d \}$ \newline
$ce^{+} = \{c, e \}$ \newline
$de^{+} = \{a, c, d, e \}$ \newline
$\Rightarrow keys: \{b, d\}, \{b, c\}$ 

\section{Task}
$R(a, b, c, d)$ with $F_{R} = \{ ab \rightarrow c, c \rightarrow d, d \rightarrow a \}$ \newline
$S(a, b, c, d)$ with $F_{R} = \{ a \rightarrow b, b \rightarrow c, b \rightarrow d \}$

$R^{+} = \{ 
            ab \rightarrow a,
            ab \rightarrow c,
            ab \rightarrow d,
            c \rightarrow a,
            c \rightarrow d,
            cd \rightarrow d,
            d \rightarrow a
        \}$

$S^{+} = \{
            a \rightarrow b,
            a \rightarrow c, 
            a \rightarrow d, 
            b \rightarrow c, 
            b \rightarrow d
        \}$
\newpage
\section{Task}
$R(a, b, c, d)$ with $F = \{ ab \rightarrow c, bc \rightarrow d, b \rightarrow d, ad \rightarrow b \}$\newline
$R_{1}(a, b, c)$  \newline
$R_{2}(b, d)$ \newline
$R_{3}(a, b, c)$ \newline
$R_{4}(a, b, d)$ \newline

\begin{enumerate}
    \item 
    $R_{1} \cap R_{2} = b$ \newline
    $b^{+} = \{b, d\} = R_{2} \Rightarrow $ lossless

    $F_{1} = \{ab \rightarrow c\}$ \newline
    $F_{2} = \{b \rightarrow d\}$ \newline
    $(F_{1} \cup F_{2})^{+} = $
    $\Rightarrow$ not dependency preserving
    \item 
    $R_{3} \cap R_{4} = b$ \newline
    $b^{+} = \{b, d\} \neq R_{3}$ \newline
    $b^{+} = \{b, d\} \neq R_{4} \Rightarrow $ lossy

    $F_{3} = \{ab \rightarrow c\}$ \newline
    $F_{4} = \{b \rightarrow d, ad \rightarrow b \}$ \newline
    $(F_{3} \cup F_{4})^{+} 
    = (\{ab \rightarrow c\} \cup \{b \rightarrow d, ad \rightarrow b \})^{+} 
    = (\{ab \rightarrow c, b \rightarrow d, ad \rightarrow b , bc \rightarrow d\} )^{+} 
    = F^{+}$ \newline
    $ \Rightarrow(F_{3} \cup F_{4})^{+} = F^{+}$
    $\Rightarrow$ dependency preserving
\end{enumerate}

\end{document}
